coqimp/example/code/code.v
@@ -1,0 +1,159 @@
+Require Import Coqlib.       
+Require Import Maps.      
+Require Import LibTactics.  
+       
+Require Import Integers.  
+Open Scope Z_scope.    
+Import ListNotations.
+  
+Set Asymmetric Patterns.  
+       
+Require Import state.    
+Require Import language. 
+
+Set Implicit Arguments.  
+Unset Strict Implicit. 
+             
+Require Import logic.
+   
+Require Import lemmas.
+Require Import lemmas_ins.
+
+Require Import Coq.Logic.FunctionalExtensionality.
+  
+Open Scope nat.
+Open Scope code_scope.
+Open Scope mem_scope.
+
+(** context offset *)
+Definition OS_L0_OFFSET := ($ 0).
+Definition OS_L1_OFFSET := ($ 4).
+Definition OS_L2_OFFSET := ($ 8).
+Definition OS_L3_OFFSET := ($ 12).
+
+Definition OS_I0_OFFSET := ($ 16).
+Definition OS_I1_OFFSET := ($ 20).
+Definition OS_I2_OFFSET := ($ 24).
+Definition OS_I3_OFFSET := ($ 28).
+Definition OS_I4_OFFSET := ($ 32).
+Definition OS_I5_OFFSET := ($ 36).
+Definition OS_I6_OFFSET := ($ 40).
+Definition OS_I7_OFFSET := ($ 44).
+
+Definition OS_G0_OFFSET := ($ 48).
+Definition OS_G1_OFFSET := ($ 52).
+Definition OS_G2_OFFSET := ($ 56).
+Definition OS_G3_OFFSET := ($ 60).
+Definition OS_G4_OFFSET := ($ 64).
+Definition OS_G5_OFFSET := ($ 68).
+Definition OS_G6_OFFSET := ($ 72).
+Definition OS_G7_OFFSET := ($ 76).
+
+Definition OS_Y_OFFSET := ($ 80).
+
+(** stack offset *)
+Definition OS_CPU_STACK_FRAME_L0_OFFSET := ($ 0).
+Definition OS_CPU_STACK_FRAME_L1_OFFSET := ($ 4).
+Definition OS_CPU_STACK_FRAME_L2_OFFSET := ($ 8).
+Definition OS_CPU_STACK_FRAME_L3_OFFSET := ($ 12).
+Definition OS_CPU_STACK_FRAME_L4_OFFSET := ($ 16).
+Definition OS_CPU_STACK_FRAME_L5_OFFSET := ($ 20).
+Definition OS_CPU_STACK_FRAME_L6_OFFSET := ($ 24).
+Definition OS_CPU_STACK_FRAME_L7_OFFSET := ($ 28).
+
+Definition OS_CPU_STACK_FRAME_I0_OFFSET := ($ 32).
+Definition OS_CPU_STACK_FRAME_I1_OFFSET := ($ 36).
+Definition OS_CPU_STACK_FRAME_I2_OFFSET := ($ 40).
+Definition OS_CPU_STACK_FRAME_I3_OFFSET := ($ 44).
+Definition OS_CPU_STACK_FRAME_I4_OFFSET := ($ 48).
+Definition OS_CPU_STACK_FRAME_I5_OFFSET := ($ 52).
+Definition OS_CPU_STACK_FRAME_I6_OFFSET := ($ 56).
+Definition OS_CPU_STACK_FRAME_I7_OFFSET := ($ 60).
+
+(** TCB offset *)
+Definition OS_CONTEXT_OFFSET := ($ 84).
+
+(** WINDOW count *)
+Definition OS_WINDOWS := ($ 8).
+
+(** Variable *)
+Definition OSTRUE := ($ 1).
+Definition OSFALSE := ($ 0).
+
+(** Code Notation *)
+Definition g0 := r0.
+Definition g1 := r1.
+Definition g2 := r2.
+Definition g3 := r3.
+Definition g4 := r4.
+Definition g5 := r5.
+Definition g6 := r6.
+Definition g7 := r7.
+
+Definition o0 := r8.
+Definition o1 := r9.
+Definition o2 := r10.
+Definition o3 := r11.
+Definition o4 := r12.
+Definition o5 := r13.
+Definition o6 := r14.
+Definition o7 := r15.
+
+Definition l0 := r16.
+Definition l1 := r17.
+Definition l2 := r18.
+Definition l3 := r19.
+Definition l4 := r20.
+Definition l5 := r21.
+Definition l6 := r22.
+Definition l7 := r23.
+
+Definition i0 := r24.
+Definition i1 := r25.
+Definition i2 := r26.
+Definition i3 := r27.
+Definition i4 := r28.
+Definition i5 := r29.
+Definition i6 := r30.
+Definition i7 := r31.
+
+Definition sp := r14.
+
+Notation "' n" := (Ow ($ n)) (at level 10) : code_scope.
+
+Notation "'[' rn ']ₓ'" := (Ao (Or rn)) (at level 10) : code_scope.
+
+(** label *)
+Definition f := ($ 324).
+Definition changeY := ($ 480).
+
+Definition funcadd : InsSeq :=
+  add i0 (Or i1) l7 ;;
+  add l7 (Or i2) l7 ;;
+  retl ;;
+  nop.
+
+Definition funChangeY : InsSeq :=
+  rd Ry l0 ;;
+  wr i0 (Ow ($ 0)) Ry ;;
+  nop ;;
+  nop ;;
+  nop ;;
+  restore l0 (Ow ($ 0)) o0 ;;
+  retl ;;
+  nop.
+
+Definition Caller : InsSeq :=
+  add g0 (Ow ($ 1)) o0 ;;
+  call changeY #
+  save sp (Ow (Int.neg ($ 64))) sp #
+  add g0 (Or o0) l0 ;;
+  retl ;;
+  nop.
+
+Definition sum3_1 : InsSeq :=
+  save sp (Ow (Int.neg ($ 64))) sp ;;
+  add i0 (Or i1) l7 ;;
+  add l7 (Or i2) l7 ;;
+  ret ;;
+  restore l7 (Ow ($ 0)) o0.
