coqimp/example/lib/tm_dly_lemma.v
@@ -1,0 +1,346 @@
+Require Import Coqlib.                         
+Require Import Maps.           
+Require Import LibTactics.   
+        
+Require Import Integers.  
+Open Scope Z_scope.        
+Import ListNotations.  
+   
+Set Asymmetric Patterns.  
+        
+Require Import state.    
+Require Import language. 
+ 
+Set Implicit Arguments.    
+Unset Strict Implicit. 
+               
+Require Import logic.
+    
+Require Import lemmas.
+Require Import lemmas_ins.
+
+Require Import Coq.Logic.FunctionalExtensionality.
+
+Require Import sep_lemma.
+Require Import reg_lemma.
+
+Open Scope nat.
+Open Scope code_scope.
+Open Scope mem_scope.
+
+(*+ Operation for TimeReduce +*)
+(* Delay Time Reduce *)
+Fixpoint TimReduce (a : asrt) : asrt :=
+  match a with
+  | p //\\ q => (TimReduce p) //\\ (TimReduce q)
+  | p \\// q => (TimReduce p) \\// (TimReduce q)
+  | p ** q => (TimReduce p) ** (TimReduce q)
+  | Aforall t p => Aforall (fun x : t => (TimReduce (p x)))
+  | Aexists t p => Aexists (fun x : t => (TimReduce (p x)))
+  | Aregdly t rsp v =>
+    match t with
+    | O => rsp |=> v
+    | S t' => t' @ rsp |==> v
+    end
+  | ATimReduce p => ATimReduce (TimReduce p)
+  | _ => a
+  end.
+
+Theorem asrt_time_reduce' :
+  forall p M R R' F D D',
+    (M, (R, F), D) |= p -> (R', D') = exe_delay R D ->
+    (M, (R', F), D') |= TimReduce p.
+Proof.
+  intro p. 
+  induction p; intros;
+    try solve [simpls; simpljoin1; eauto]; simpl TimReduce.
+  -
+    eapply dly_reduce_Aemp_stable; eauto.
+  -
+    eapply dly_reduce_Amapsto_stable; eauto.
+  -
+    eapply dly_reduce_Aaexp_stable; eauto.
+  -
+    eapply dly_reduce_Aoexp_stable; eauto.
+  -
+    eapply dly_reduce_reg_stable; eauto.
+  -
+    destruct n.
+    eapply dlytime_zero_exe_dly; eauto.
+    eapply dlytime_gt_zero_reduce_exe_dly; eauto.
+  -
+    eapply dly_reduce_pure_stable; eauto.
+  -
+    eapply Afrmlist_exe_delay_stable; eauto.
+  -
+    simpl in H.
+    destruct H; eauto.
+    simpl; eauto.
+    simpl; eauto.
+  -
+    sep_star_split_tac.
+    simpls.
+    simpljoin1.
+    symmetry in H0.
+    eapply exe_dly_sep_split in H0; eauto.
+    simpljoin1.
+    eapply IHp1 in H; eauto.
+    eapply IHp2 in H3; eauto.
+    exists (m, (x, f0), D') (m0, (x0, f0), D').
+    simpls; eauto.
+    repeat (split; eauto).
+Qed.
+
+Theorem asrt_time_reduce :
+  forall S p,
+    S |= p ↓ -> S |= TimReduce p.
+Proof.
+  intros.
+  simpl in H.
+  simpljoin1.
+  destruct_state S.
+  simpls.
+  eapply asrt_time_reduce'; eauto.
+Qed.
+
+(*+ Lemmas about TimReduce +*)
+Theorem astar_TimReduce :
+  forall p q,
+    TimReduce (p ** q) = (TimReduce p) ** (TimReduce q).
+Proof.
+  intros; simpl; eauto.
+Qed.
+
+Theorem Regs_TimeReduce :
+  forall fmo fml fmi p,
+    TimReduce (Regs fmo fml fmi ** p) = Regs fmo fml fmi ** (TimReduce p).
+Proof.
+  intros.
+  simpl.
+  unfold Regs, OutRegs, LocalRegs, InRegs.
+  destruct fmo, fml, fmi.
+  simpl.
+  eauto.
+Qed.
+  
+Theorem GenRegs_TimeReduce :
+  forall grst p,
+    TimReduce (GenRegs grst ** p) = GenRegs grst ** (TimReduce p).
+Proof.
+  intros.
+  simpl.
+  destruct grst.
+  destruct p0.
+  destruct p0.
+  destruct f1, f2, f0, f.
+  simpl.
+  eauto.
+Qed.
+
+Theorem GenRegs_rm_one_TimReduce' :
+  forall grst (rr : GenReg) ,
+    TimReduce (GenRegs_rm_one grst rr) = GenRegs_rm_one grst rr.
+Proof. 
+  intros.
+  simpl.
+  destruct grst.
+  destruct p.
+  destruct p.
+  destruct f1, f2, f0, f.
+  simpls.
+  destruct rr; simpls; eauto.
+Qed.
+
+Theorem GenRegs_rm_one_TimReduce :
+  forall grst (rr : GenReg) p,
+    TimReduce (GenRegs_rm_one grst rr ** p) = GenRegs_rm_one grst rr ** (TimReduce p).
+Proof.
+  intros.
+  simpl.
+  rewrite GenRegs_rm_one_TimReduce'; eauto.
+Qed.
+
+Theorem RegSt_TimeReduce :
+  forall rn v p,
+    TimReduce (rn |=> v ** p) = rn |=> v ** (TimReduce p).
+Proof.
+  intros.
+  simpl; eauto.
+Qed.
+
+Theorem MemSto_TimeReduce :
+  forall l v p,
+    TimReduce (l |-> v ** p) = l |-> v ** (TimReduce p).
+Proof.
+  intros.
+  simpl; eauto.
+Qed.
+
+Theorem conj_TimeReduce :
+  forall p1 p2,
+    TimReduce (p1 //\\ p2) = (TimReduce p1) //\\ (TimReduce p2).
+Proof.
+  intros; eauto.
+Qed.
+
+Theorem disj_TimeReduce :
+  forall p1 p2,
+    TimReduce (p1 \\// p2) = (TimReduce p1) \\// (TimReduce p2).
+Proof.
+  intros; eauto.
+Qed.
+
+Theorem pure_TimeReduce :
+  forall pu p,
+    TimReduce ([| pu |] ** p) = [| pu |] ** (TimReduce p).
+Proof.
+  intros; eauto.
+Qed.
+
+Theorem Atrue_TimeReduce :
+  forall p,
+    TimReduce (Atrue ** p) = Atrue ** (TimReduce p).
+Proof.
+  intros; eauto.
+Qed.
+
+Theorem Afalse_TimReduce :
+  forall p,
+    TimReduce (Afalse ** p) = Afalse ** (TimReduce p).
+Proof.
+  intros; eauto.
+Qed.
+
+Theorem tmreduce_TimReduce :
+  forall p,
+    TimReduce (p ↓) = (TimReduce p) ↓.
+Proof.
+  intros.
+  simpls.
+  eauto.
+Qed.
+
+Ltac TimReduce_simpl_bas :=
+  match goal with
+  | |- context [TimReduce (Regs ?fmo ?fml ?fmi ** ?p)] =>
+    rewrite Regs_TimeReduce; TimReduce_simpl_bas
+  | |- context [TimReduce (GenRegs ?grst ** ?p)] =>
+    rewrite GenRegs_TimeReduce; TimReduce_simpl_bas
+  | |- context [TimReduce (GenRegs_rm_one ?grst ?rr ** ?p)] =>
+    rewrite GenRegs_rm_one_TimReduce; TimReduce_simpl_bas
+  | |- context [TimReduce (?rn |=> ?v ** ?p)] =>
+    rewrite RegSt_TimeReduce; TimReduce_simpl_bas
+  | |- context [TimReduce (?l |-> ?v ** ?p)] =>
+    rewrite MemSto_TimeReduce; TimReduce_simpl_bas
+  | |- context [TimReduce ([| ?pu |] ** ?p)] =>
+    rewrite pure_TimeReduce; TimReduce_simpl_bas
+  | |- context [TimReduce (Atrue ** ?p)] =>
+    rewrite Atrue_TimeReduce; TimReduce_simpl_bas
+  | |- context [TimReduce (Afalse ** ?p)] =>
+    rewrite Afalse_TimReduce; TimReduce_simpl_bas
+  | |- context [TimReduce (GenRegs_rm_one ?grst ?rr)] =>
+    rewrite GenRegs_rm_one_TimReduce'; TimReduce_simpl_bas
+  | |- context [TimReduce (?p1 //\\ ?p2)] =>
+    rewrite conj_TimeReduce; TimReduce_simpl_bas
+  | |- context [TimReduce (?p1 \\// ?p2)] =>
+    rewrite disj_TimeReduce; TimReduce_simpl_bas
+  | |- context [TimReduce (?p1 ** ?p2)] =>
+    rewrite astar_TimReduce; TimReduce_simpl_bas
+  | |- context [TimReduce (?p ↓)] =>
+    rewrite tmreduce_TimReduce; TimReduce_simpl_bas
+  | _ => simpl TimReduce
+  end.
+
+Ltac ins_tm_reduce_bas :=
+  match goal with
+  | |- |- {{ _ ↓ }} _ {{ _ }} =>
+    eapply ins_conseq_rule;
+    [
+      let H := fresh in
+      introv H; eapply asrt_time_reduce in H; eauto | eauto..
+    ]; try TimReduce_simpl_bas
+  | _ => idtac
+  end.
+
+Ltac TimReduce_simpl_in_bas H :=
+  match type of H with
+  | _ |= ?p =>
+    match p with
+    | context [TimReduce (Regs ?fmo ?fml ?fmi ** ?p)] =>
+      rewrite Regs_TimeReduce in H; TimReduce_simpl_in_bas H
+    | context [TimReduce (GenRegs ?grst ** ?p)] =>
+      rewrite GenRegs_TimeReduce in H; TimReduce_simpl_bas H
+    | context [(?rn |=> ?v ** ?p) ↓] =>
+      rewrite RegSt_TimeReduce in H; TimReduce_simpl_in_bas H
+    | context [(?l |-> ?v ** ?p) ↓] =>
+      rewrite MemSto_TimeReduce in H; TimReduce_simpl_in_bas H
+    | context [([| ?pu |] ** ?p) ↓] =>
+      rewrite pure_TimeReduce in H; TimReduce_simpl_in_bas H
+    | context [(Atrue ** ?p) ↓] =>
+      rewrite Atrue_TimeReduce in H; TimReduce_simpl_in_bas H
+    | context [(Afalse ** ?p) ↓] =>
+      rewrite Afalse_TimReduce in H; TimReduce_simpl_in_bas H
+    | context [(?p1 //\\ ?p2) ↓] =>
+      rewrite conj_TimeReduce in H; TimReduce_simpl_in_bas H
+    | context [(?p1 \\// ?p2) ↓] =>
+      rewrite disj_TimeReduce in H; TimReduce_simpl_in_bas H
+    | context [TimReduce (?p ↓)] =>
+      rewrite tmreduce_TimReduce in H; TimReduce_simpl_bas H
+    | _ => simpl TimReduce in H
+    end
+  end.
+
+(*+ Lemmas about DlyFrameFree +*)
+Lemma Atrue_DlyFrameFree :
+  forall p,
+    DlyFrameFree p -> DlyFrameFree (Atrue ** p).
+Proof.
+  intros.
+  simpl; eauto.
+Qed.
+
+Lemma Afalse_DlyFrameFree :
+  forall p,
+    DlyFrameFree p -> DlyFrameFree (Afalse ** p).
+Proof.
+  intros.
+  simpl; eauto.
+Qed.
+
+Lemma RegSt_DlyFrameFree :
+  forall rn v p,
+    DlyFrameFree p -> DlyFrameFree (rn |=> v ** p).
+Proof.
+  intros.
+  simpl; eauto.
+Qed.
+
+Lemma MapSto_DlyFrameFree :
+  forall l v p,
+    DlyFrameFree p -> DlyFrameFree (l |-> v ** p).
+Proof.
+  intros.
+  simpl; eauto.
+Qed.
+
+Lemma astar_DlyFrameFree :
+  forall p1 p2,
+    DlyFrameFree p1 -> DlyFrameFree p2 -> DlyFrameFree (p1 ** p2).
+Proof.
+  intros.
+  simpl; eauto.
+Qed.
+  
+Ltac DlyFrameFree_elim_bas :=
+  match goal with
+  | |- DlyFrameFree (Atrue ** ?p) =>
+    eapply Atrue_DlyFrameFree; DlyFrameFree_elim_bas
+  | |- DlyFrameFree (Afalse ** ?p) =>
+    eapply Afalse_DlyFrameFree; DlyFrameFree_elim_bas
+  | |- DlyFrameFree (?rn |=> ?v ** ?p) =>
+    eapply RegSt_DlyFrameFree; DlyFrameFree_elim_bas
+  | |- DlyFrameFree (?l |-> ?v ** ?p) =>
+    eapply MapSto_DlyFrameFree; DlyFrameFree_elim_bas
+  | _ =>
+    try solve [simpl; eauto]
+  end.
