coqimp/example/proof/ChangeYProof.v
@@ -1,0 +1,169 @@
+Require Import Coqlib.        
+Require Import Maps.            
+Require Import LibTactics.   
+        
+Require Import Integers.  
+Open Scope Z_scope.        
+Import ListNotations.  
+   
+Set Asymmetric Patterns.  
+        
+Require Import state.    
+Require Import language.  
+ 
+Set Implicit Arguments.    
+Unset Strict Implicit. 
+               
+Require Import logic.
+    
+Require Import lemmas.
+Require Import lemmas_ins.
+
+Require Import Coq.Logic.FunctionalExtensionality.
+
+Require Import integer_lemma.
+
+Require Import sep_lemma.
+Require Import reg_lemma.
+Require Import derived_rule.
+
+Require Import tm_dly_lemma.
+
+Require Import code.
+Require Import spec.
+
+Open Scope nat.
+Open Scope code_scope.
+Open Scope mem_scope.
+
+Definition spec := convert_spec nil.
+
+Lemma get_frm_nth_to_nth' :
+  forall fm n x,
+    get_frame_nth fm n = Some x ->
+    get_frame_nth' fm n = x.
+Proof.
+  intros.
+  destruct fm.
+  do 8
+     (destruct n; simpls;
+      inversion H; eauto).
+Qed.
+
+Lemma frm_get_upd :
+  forall fm n x,
+    0 <= n <= 7 -> 
+    get_frame_nth' (update_frame fm n x) n = x.
+Proof.
+  intros.
+  destruct fm.
+  do 8 (destruct n; simpl; eauto).
+  omega.
+Qed.
+
+Theorem ChangeYProof :
+  forall vl,
+    spec |- {{ changeY_pre vl }}
+             f # funChangeY
+           {{ changeY_post vl }}.
+Proof.
+  intros.
+  unfold changeY_pre.
+  unfold changeY_post.  
+  hoare_ex_intro_pre.
+  renames x' to fmg, x'0 to fmo, x'1 to fml, x'2 to fmi.
+  renames x'5 to vy, x'6 to vi, x'7 to id, x'8 to fm1, x'9 to fm2, x'10 to F.
+  renames x'3 to fret, x'4 to x.
+  eapply Pure_intro_rule; intros.
+
+  hoare_lift_pre 5.
+  eapply Pure_intro_rule.
+  introv Hpure.
+  simpljoin1.
+
+  unfold funChangeY.
+
+  (** rd Ry l0 *)
+  eapply seq_rule.
+  ins_tm_reduce_bas.
+  eapply rd_rule_reg; eauto.
+  simpl upd_genreg.
+
+  (** wr i0 0 Ry *)
+  eapply seq_rule.
+  ins_tm_reduce_bas.
+  eapply wr_rule_reg; eauto.
+  simpl.
+  rewrite in_range0; eauto.
+  simpl set_spec_reg.
+  rewrite Int.xor_zero.
+
+  (** nop *)
+  eapply seq_rule.
+  ins_tm_reduce_bas.
+  eapply nop_rule; eauto.
+
+  (** nop *)
+  eapply seq_rule.
+  ins_tm_reduce_bas.
+  eapply nop_rule; eauto.
+
+  (** nop *)
+  eapply seq_rule.
+  ins_tm_reduce_bas.
+  eapply nop_rule; eauto.
+
+  (** restore l0 0 o0 *)
+  hoare_lift_pre 4.
+  hoare_lift_pre 4.
+  hoare_lift_pre 3.
+  eapply seq_rule.
+  ins_tm_reduce_bas.
+  eapply restore_rule_reg; eauto.
+  simpl.
+  rewrite in_range0; eauto.
+  simpl upd_genreg.
+  rewrite Int.add_zero.
+
+  (** retl ;; nop *)
+  eapply retl_rule.
+  ins_tm_reduce_bas.
+  ins_tm_reduce_bas.
+  eapply nop_rule; eauto.
+
+  introv Hs.
+  sep_ex_intro. 
+  sep_cancel1 1 2.
+  sep_cancel1 3 2.
+  sep_cancel1 1 2.
+  sep_cancel1 1 2.
+  instantiate (1 := Aemp).
+  eapply astar_emp_intro_r.
+  eauto.
+  eapply sep_pure_l_intro.
+  eauto. 
+  erewrite get_frm_nth_to_nth'.
+  rewrite frm_get_upd; eauto.
+  omega.
+  eauto.
+  eauto.
+  unfold fretSta.
+  introv Hs Hs'.
+  eapply asrt_time_reduce in Hs.
+  rewrite tmreduce_TimReduce in Hs.
+  eapply asrt_time_reduce in Hs.
+  do 2 rewrite GenRegs_TimeReduce in Hs.
+  TimReduce_simpl_in_bas Hs.
+
+  eapply GenRegs_split_one with (rr := r15) in Hs.
+  simpl get_genreg_val' in Hs.
+  eapply GenRegs_split_one with (rr := r15) in Hs'.
+  simpl get_genreg_val' in Hs'.
+  clear - Hs Hs'.
+  destruct_state s.
+  destruct_state s'.
+  eapply rn_st_v_eval_reg_v in Hs.
+  eapply rn_st_v_eval_reg_v in Hs'.
+  simpl.
+  eauto.
+Qed.
