coqimp/example/proof/FunAddProof.v
@@ -1,0 +1,135 @@
+Require Import Coqlib.                                                                    
+Require Import Maps.            
+Require Import LibTactics.   
+        
+Require Import Integers.  
+Open Scope Z_scope.        
+Import ListNotations.  
+   
+Set Asymmetric Patterns.  
+        
+Require Import state.    
+Require Import language.  
+ 
+Set Implicit Arguments.    
+Unset Strict Implicit. 
+               
+Require Import logic.
+    
+Require Import lemmas.
+Require Import lemmas_ins.
+
+Require Import Coq.Logic.FunctionalExtensionality.
+
+Require Import integer_lemma.
+
+Require Import sep_lemma.
+Require Import reg_lemma.
+Require Import derived_rule.
+
+Require Import tm_dly_lemma.
+
+Require Import code.
+Require Import spec.
+
+Open Scope nat.
+Open Scope code_scope.
+Open Scope mem_scope.
+
+Definition spec := convert_spec nil.
+
+Theorem FunAddProof :
+  forall vl,
+    spec |- {{ add_pre vl }}
+             f # funcadd
+           {{ add_post vl }}.
+Proof.
+  intros.
+  unfold add_pre.
+  unfold add_post.
+  hoare_ex_intro_pre.
+  renames x' to x, x'0 to y, x'1 to z, x'3 to fret.
+  eapply Pure_intro_rule; intros.
+  unfold funcadd.
+
+  (** add i0 i1 l7 *)
+  eapply seq_rule.
+  ins_tm_reduce_bas.
+  eapply add_rule; eauto.
+  introv Hs.
+  split.
+  {
+    destruct_state s.
+    eapply rn_st_v_eval_reg_v in Hs.
+    simpl; eauto.
+    unfold get_R.
+    simpl; eauto.
+    rewrite Hs; eauto.
+  }
+  {
+    simpl_sep_liftn_in Hs 2.
+    destruct_state s.
+    eapply rn_st_v_eval_reg_v in Hs; eauto.
+    simpl; eauto.
+    unfold get_R.
+    simpl; eauto.
+    rewrite Hs; eauto.
+  }
+  introv Hs.
+  simpl_sep_liftn_in Hs 4; eauto.
+
+  (** add l7 i2 l7 *)
+  eapply seq_rule.
+  ins_tm_reduce_bas.
+  eapply add_rule; eauto.
+  introv Hs.
+  split.
+  {
+    destruct_state s.
+    eapply rn_st_v_eval_reg_v in Hs; eauto.
+    simpl.
+    unfold get_R.
+    simpl; eauto.
+    rewrite Hs; eauto.
+  }
+  {
+    simpl_sep_liftn_in Hs 4.
+    destruct_state s.
+    eapply rn_st_v_eval_reg_v in Hs.
+    simpl.
+    unfold get_R.
+    simpl; eauto.
+    rewrite Hs; eauto.
+  }
+
+  (** retl ;; nop *)
+  eapply retl_rule; eauto.
+  ins_tm_reduce_bas.
+  ins_tm_reduce_bas.
+  eapply nop_rule; eauto.
+  introv Hs.
+  sep_ex_intro.
+  eapply sep_pure_l_intro; eauto.
+  sep_cancel1 2 1.
+  sep_cancel1 2 1.
+  sep_cancel1 2 1.
+  eauto.
+
+  unfold fretSta.
+  introv Hs Hs'.
+  eapply asrt_time_reduce in Hs.
+  TimReduce_simpl_in_bas Hs.
+  eapply asrt_time_reduce in Hs.
+  TimReduce_simpl_in_bas Hs.
+  simpl_sep_liftn_in Hs 5.
+  sep_ex_elim_in Hs'. 
+  eapply sep_pure_l_elim in Hs'.
+  simpljoin1.
+  symmetry in H0.
+  inversion H0; eauto; subst.
+  simpl_sep_liftn_in H1 5.
+  destruct_state s.
+  eapply rn_st_v_eval_reg_v in Hs; eauto.
+  destruct_state s'.
+  eapply rn_st_v_eval_reg_v in H1; eauto.
+Qed.
