coqimp/example/proof/Sum3Proof.v
@@ -1,0 +1,165 @@
+Require Import Coqlib.                                                                             
+Require Import Maps.            
+Require Import LibTactics.   
+        
+Require Import Integers.  
+Open Scope Z_scope.        
+Import ListNotations.  
+   
+Set Asymmetric Patterns.  
+        
+Require Import state.    
+Require Import language.  
+ 
+Set Implicit Arguments.    
+Unset Strict Implicit. 
+               
+Require Import logic.
+    
+Require Import lemmas.
+Require Import lemmas_ins.
+
+Require Import Coq.Logic.FunctionalExtensionality.
+
+Require Import integer_lemma.
+
+Require Import sep_lemma.
+Require Import reg_lemma.
+Require Import derived_rule.
+
+Require Import tm_dly_lemma.
+
+Require Import code.
+Require Import spec.
+
+Open Scope nat.
+Open Scope code_scope.
+Open Scope mem_scope.
+
+Definition spec := convert_spec nil.
+
+Lemma inrange_neg_64 :
+  ($ (-4096)) <=ᵢ (Int.neg $ 64) && (Int.neg $ 64) <=ᵢ ($ 4095) = true.
+Proof.
+  eauto.
+Qed.
+
+Theorem Sum3Proof1 :
+  forall vl,
+    spec |- {{ sum3_pre1 vl }}
+             f # sum3_1
+            {{ sum3_post1 vl }}.
+Proof.
+  intros.
+  unfold sum3_pre1.
+  unfold sum3_post1.
+  hoare_ex_intro_pre.
+  renames x' to x, x'0 to y, x'1 to z, x'2 to fret.
+  renames x'3 to fmg, x'4 to fmo, x'5 to fml, x'6 to fmi.
+  renames x'7 to id, x'8 to vi, x'9 to F, x'10 to fm1, x'11 to fm2. 
+  eapply Pure_intro_rule; intros.
+
+  hoare_lift_pre 4.
+  eapply Pure_intro_rule.
+  introv Hpure.
+  simpljoin1.
+
+  unfold sum3_1.
+
+  (** save sp, -64, sp *)
+  eapply seq_rule.
+  ins_tm_reduce_bas.
+  eapply save_rule_reg; eauto.
+  simpl.
+  rewrite inrange_neg_64.
+  eauto.
+  simpl upd_genreg.
+  
+  (** add i0 i1 l7 *) 
+  destruct fm2, fmo.
+  simpl get_frame_nth'.
+  eapply seq_rule.
+  ins_tm_reduce_bas. 
+  eapply add_rule_reg; eauto.
+  simpl upd_genreg.
+
+  (** add l7 i2 l7 *)
+  eapply seq_rule.
+  ins_tm_reduce_bas.
+  eapply add_rule_reg; eauto.
+  simpl upd_genreg.
+
+  (** ret ;; restore l7 0 o0  *)
+  eapply ret_rule; eauto.
+  ins_tm_reduce_bas.
+  ins_tm_reduce_bas.
+  eapply ins_conseq_rule.
+  eauto.
+  eapply restore_rule_reg; eauto.
+  simpl.
+  rewrite in_range0; eauto.
+  rewrite post_pre_stable; eauto.
+  simpl upd_genreg.
+  introv Hs.
+  sep_ex_intro.
+  sep_cancel1 1 2.
+  sep_cancel1 1 2.
+  sep_cancel1 1 2.
+  instantiate (1 := Aemp).
+  eapply astar_emp_intro_r; eauto.
+  eapply sep_pure_l_intro.
+  eauto.
+  match goal with
+  | H : _ |= _ |- _ => rename H into Hs
+  end.
+  simpl in Hs.
+  simpl.
+  simpljoin1.
+  repeat (split; eauto).
+
+  rename H0 into Ho0.
+  simpl in Ho0.
+  inversion Ho0; subst.
+  rewrite Int.add_assoc.
+  rewrite Int.add_zero.
+  eauto.
+  rewrite post_pre_stable; eauto.
+  rewrite post_pre_stable; eauto.
+  eapply in_range_0_7_post_cwp_still; eauto.
+  eapply in_range_0_7_pre_cwp_still; eauto.
+
+  unfold fretStoreSta.
+  introv Hs Hs'.
+  eapply asrt_time_reduce in Hs.
+  rewrite tmreduce_TimReduce in Hs.
+  eapply asrt_time_reduce in Hs.
+  do 2 rewrite GenRegs_TimeReduce in Hs.
+  TimReduce_simpl_in_bas Hs.
+
+  eapply GenRegs_split_one with (rr := r31) in Hs.
+  simpl get_genreg_val' in Hs.
+  simpl in H3.
+  inversion H3; subst.
+  sep_ex_elim_in Hs'.
+  eapply sep_pure_l_elim in Hs'.
+  destruct Hs' as [Hlgvl1 Hs'].
+  inversion Hlgvl1; subst.
+  simpl_sep_liftn_in Hs' 4.
+  eapply sep_pure_l_elim in Hs'.
+  destruct Hs' as [Hpure Hs'].
+  simpljoin1.
+  eapply GenRegs_split_one with (rr := r15) in Hs'.
+  simpl get_genreg_val' in Hs'.
+  destruct x5.
+  simpl get_frame_nth' in Hs'.
+  simpl in H7.
+  inversion H7; subst.
+  clear - Hs Hs'.
+  destruct_state s.
+  destruct_state s'.
+  eapply rn_st_v_eval_reg_v in Hs.
+  eapply rn_st_v_eval_reg_v in Hs'.
+  eexists.
+  simpl.
+  split; eauto.
+Qed.
